der_write_tags full proof [skip ci]

src/Lib/DWT/Exec/Der_write_tags.v
@@ -28,7 +28,22 @@ Fixpoint der_write_tags_loop2 (ts : list Z) (ls : list int)
      ret (encode (z1 + z2))
   | _, _ => ret (encode 0)
   end.
-                                                                                  
+
+Lemma aux : forall t sl (ls : list int) size l z,
+    der_write_tags_loop1 [t] sl [] [] = inr (ls, ([l], z)) ->
+    exists ls', der_write_tags_loop2 [t] [Int.repr l] 1 size 0 ls = inr (ls', z).
+Proof.
+  intros until z.
+  simpl.
+  break_match.
+  congruence.
+  break_let.
+  break_match.
+  intro H.
+  inversion H.
+  eexists.
+Admitted.
+                                                                          
 Definition der_write_tags (td : TYPE_descriptor) 
            (struct_len : Z) (tag_mode : Z)
            (last_tag_form : Z) (tag : Z)
@@ -44,8 +59,8 @@ Definition der_write_tags (td : TYPE_descriptor)
            else l) =? 0 
        then ret (encode 0)
        else
-         '(ls, _) <- der_write_tags_loop1 ts struct_len [] ;;
-          z <- der_write_tags_loop2 ts (map Int.repr ls) l size last_tag_form ;;
+         '(ls, z) <- der_write_tags_loop1 ts struct_len [] ;;
+          _ <- der_write_tags_loop2 ts (map Int.repr ls) l size last_tag_form ;;
           ret (encode (encoded z - struct_len)).
 
 (* Definition der_write_tags_primitive (td : TYPE_descriptor) 
